feature(wasm) cleaner treatment of foreign data/ops support in WASM
Signed-off-by: Jerome Simeon <jeromesimeon@me.com>

compiler/wasm/wasm_enhanced.ml
@@ -1,5 +1,9 @@
-let foreign_ejson_to_wson fdata =
+let foreign_ejson_to_wson x =
   failwith "Wasm_enhanced.foreign_ejson_to_wasm: Do not know how to convert foreign EJson to Wasm"
 
+let foreign_wson_to_ejson x =
+  failwith "Wasm_enhanced.foreign_wson_to_ejson: Do not know how to convert foreign Wasm to EJson"
+    
 let foreign_ejson_to_wasm_op fop =
   failwith "Wasm_enhanced.foreign_ejson_to_wasm_op: Do not know how to convert foreign EJson to Wasm"
+
