compiler/core/Compiler/Trivial/TrivialModel.v
@@ -351,10 +351,15 @@ Next Obligation.
   destruct fd. 
 Defined.
 
-Program Instance trivial_foreign_to_wson : foreign_to_wson _
-  := mk_foreign_to_wson trivial_foreign_ejson_model _.
+Definition trivial_foreign_wson_model := Empty_set.
+
+Program Instance trivial_foreign_to_wson : foreign_to_wson _ _
+  := mk_foreign_to_wson trivial_foreign_ejson_model trivial_foreign_wson_model _ _.
 Next Obligation.
   destruct j.
+Defined.
+Next Obligation.
+  destruct fd.
 Defined.
 
 Program Instance trivial_foreign_reduce_op
@@ -396,7 +401,9 @@ Module TrivialRuntime <: CompilerRuntime.
     := trivial_foreign_ejson_runtime_op.
   Definition compiler_foreign_to_ejson : foreign_to_ejson compiler_foreign_ejson_model compiler_foreign_ejson_runtime_op
     := trivial_foreign_to_ejson.
-  Definition compiler_foreign_to_wson : foreign_to_wson compiler_foreign_ejson_model
+  Definition compiler_foreign_wson_model : Set
+    := trivial_foreign_wson_model.
+  Definition compiler_foreign_to_wson : foreign_to_wson compiler_foreign_ejson_model compiler_foreign_wson_model
     := trivial_foreign_to_wson.
   Definition compiler_foreign_to_ejson_runtime : foreign_to_ejson_runtime
     := trivial_foreign_to_ejson_runtime.
@@ -450,7 +457,9 @@ Module TrivialModel(bm:CompilerBrandModel(TrivialForeignType)) <: CompilerModel.
     := trivial_foreign_ejson_model.
   Definition compiler_model_foreign_ejson : foreign_ejson compiler_model_foreign_ejson_model
     := trivial_foreign_ejson.
-  Definition compiler_model_foreign_to_wson : foreign_to_wson compiler_model_foreign_ejson_model
+  Definition compiler_model_foreign_wson_model : Set
+    := trivial_foreign_wson_model.
+  Definition compiler_model_foreign_to_wson : foreign_to_wson compiler_model_foreign_ejson_model compiler_model_foreign_wson_model
     := trivial_foreign_to_wson.
   Definition compiler_model_foreign_ejson_runtime_op : Set
     := trivial_foreign_ejson_runtime_op.
