compiler/core/Compiler/Enhanced/EnhancedWSON.v
@@ -1,0 +1,65 @@
+(*
+ * Licensed under the Apache License, Version 2.0 (the "License");
+ * you may not use this file except in compliance with the License.
+ * You may obtain a copy of the License at
+ *
+ * http://www.apache.org/licenses/LICENSE-2.0
+ *
+ * Unless required by applicable law or agreed to in writing, software
+ * distributed under the License is distributed on an "AS IS" BASIS,
+ * WITHOUT WARRANTIES OR CONDITIONS OF ANY KIND, either express or implied.
+ * See the License for the specific language governing permissions and
+ * limitations under the License.
+ *)
+
+Require Import List.
+Require Import ZArith.
+Require Import EquivDec.
+Require Import RelationClasses.
+Require Import Equivalence.
+Require Import String.
+
+Require Import Utils.
+Require Import EJsonSystem.
+Require Import ForeignData.
+Require Import ForeignEJson.
+Require Import SqlDateComponent.
+Require Import UriComponent.
+
+Require Import EnhancedData.
+
+Import ListNotations.
+Local Open Scope list_scope.
+
+Parameter enhanced_wson : Set.
+Extract Constant enhanced_wson => "string".
+Axiom enhanced_wson_eqdec : forall x y : enhanced_wson, {x = y} + {x = y -> False}.
+Axiom enhanced_wson_normalized : forall x : enhanced_wson, Prop.
+Axiom enhanced_wson_normalize : enhanced_wson -> enhanced_wson.
+Axiom enhanced_wson_normalize_normalized : forall x : enhanced_wson, enhanced_wson_normalized (enhanced_wson_normalize x).
+Axiom enhanced_wson_normalize_idempotent : forall x : enhanced_wson, enhanced_wson_normalized x -> enhanced_wson_normalize x = x.
+Axiom enhanced_wson_to_string : enhanced_wson -> string.
+
+Program Instance enhanced_foreign_wson : foreign_ejson enhanced_wson
+  := mk_foreign_ejson enhanced_wson _ _ enhanced_wson_normalize _ _ _.
+Next Obligation.
+  red.
+  unfold equiv, complement.
+  apply enhanced_wson_eqdec.
+Defined.
+Next Obligation.
+  apply (enhanced_wson_normalized a).
+Defined.
+Next Obligation.
+  unfold enhanced_foreign_wson_obligation_2.
+  apply (enhanced_wson_normalize_normalized a).
+Defined.
+Next Obligation.
+  unfold enhanced_foreign_wson_obligation_2 in H.
+  apply enhanced_wson_normalize_idempotent.
+  assumption.
+Defined.
+Next Obligation.
+  constructor.
+  apply enhanced_wson_to_string.
+Defined.
