compiler/core/Driver/CompCorrectness.v
@@ -90,6 +90,7 @@ Require Import OptimizerLogger.
 
 (* Foreign Datatypes Support *)
 Require Import ForeignDataToEJson.
+Require Import ForeignEJsonToWSON.
 Require Import ForeignToEJsonRuntime.
 Require Import ForeignToWasmAst.
 Require Import ForeignToReduceOps.
@@ -118,6 +119,8 @@ Section CompCorrectness.
   Context {foreign_ejson_runtime_op : Set}.
   Context {ftejson:foreign_to_ejson foreign_ejson_model foreign_ejson_runtime_op}.
   Context {frtejson:foreign_to_ejson_runtime}.
+  Context {foreign_wson_model:Set}.
+  Context {ftowson:foreign_to_wson foreign_ejson_model foreign_wson_model}.
   Context {ftowasm:foreign_to_wasm_ast foreign_ejson_runtime_op}.
   Context {fredop:foreign_reduce_op}.
   Context {ftoredop:foreign_to_reduce_op}.
