compiler/core/Translation/Model/EJsonToWSON.v
@@ -1,0 +1,56 @@
+(*
+ * Licensed under the Apache License, Version 2.0 (the "License");
+ * you may not use this file except in compliance with the License.
+ * You may obtain a copy of the License at
+ *
+ * http://www.apache.org/licenses/LICENSE-2.0
+ *
+ * Unless required by applicable law or agreed to in writing, software
+ * distributed under the License is distributed on an "AS IS" BASIS,
+ * WITHOUT WARRANTIES OR CONDITIONS OF ANY KIND, either express or implied.
+ * See the License for the specific language governing permissions and
+ * limitations under the License.
+ *)
+
+Require Import List.
+Require Import Utils.
+Require Import EJsonRuntime.
+Require Import WSONRuntime.
+Require Import ForeignEJsonToWSON.
+
+Section EJsonToWSON.
+  Context {foreign_ejson_model:Set}.
+  Context {foreign_wson_model:Set}.
+  Context {ftowson:foreign_to_wson foreign_ejson_model foreign_wson_model}.
+
+  Section toWSON.
+    (* EJson to WSON *)
+    Fixpoint ejson_to_wson (j:ejson) : wson :=
+      match j with
+      | ejnull => ejnull
+      | ejnumber n => ejnumber n
+      | ejbigint n => ejbigint n
+      | ejbool b => ejbool b
+      | ejstring s => ejstring s
+      | ejarray c => ejarray (map ejson_to_wson c)
+      | ejobject r => ejobject (map (fun x => (fst x, ejson_to_wson (snd x))) r)
+      | ejforeign fd => ejforeign (foreign_to_wson_from_ejson fd)
+      end.
+  End toWSON.
+
+  Section fromWSON.
+    (* EJson to WSON *)
+    Fixpoint wson_to_ejson (j:wson) : ejson :=
+      match j with
+      | ejnull => ejnull
+      | ejnumber n => ejnumber n
+      | ejbigint n => ejbigint n
+      | ejbool b => ejbool b
+      | ejstring s => ejstring s
+      | ejarray c => ejarray (map wson_to_ejson c)
+      | ejobject r => ejobject (map (fun x => (fst x, wson_to_ejson (snd x))) r)
+      | ejforeign fd => ejforeign (foreign_to_wson_to_ejson fd)
+      end.
+  End fromWSON.
+
+End EJsonToWSON.
