compiler/core/Compiler/Model/CompilerRuntime.v
@@ -44,7 +44,8 @@ Module Type CompilerRuntime.
   Declare Instance compiler_foreign_ejson : foreign_ejson compiler_foreign_ejson_model.
   Axiom compiler_foreign_ejson_runtime_op : Set.
   Declare Instance compiler_foreign_to_ejson : foreign_to_ejson compiler_foreign_ejson_model compiler_foreign_ejson_runtime_op.
-  Declare Instance compiler_foreign_to_wson : foreign_to_wson compiler_foreign_ejson_model.
+  Axiom compiler_foreign_wson_model : Set.
+  Declare Instance compiler_foreign_to_wson : foreign_to_wson compiler_foreign_ejson_model compiler_foreign_wson_model.
   Declare Instance compiler_foreign_to_ejson_runtime : foreign_to_ejson_runtime.
   Declare Instance compiler_foreign_to_json : foreign_to_json.
   Declare Instance compiler_foreign_to_java : foreign_to_java.
